Adapt NSL proof.

nsl.v
@@ -87,7 +87,7 @@ Qed.
 
 Section NSL.
 
-Context `{!resG Σ, !heapG Σ}.
+Context `{!cryptoG Σ, !heapG Σ}.
 
 Inductive role := Init | Resp.
 
@@ -134,8 +134,8 @@ Definition swap_role rl :=
 
 Inductive session := Session {
   srole : role;
-  sinit : loc;
-  sresp : loc;
+  sinit : term;
+  sresp : term;
   sdata : option term;
 }.
 
@@ -153,7 +153,7 @@ Definition sother s :=
   if s.(srole) is Init then s.(sresp) else s.(sinit).
 
 Definition sessionR : cmraT :=
-  prodR (prodR (prodR (agreeR roleO) (agreeR locO)) (agreeR locO))
+  prodR (prodR (prodR (agreeR roleO) (agreeR termO)) (agreeR termO))
         (optionR (agreeR termO)).
 
 Implicit Types t : term.
@@ -320,7 +320,7 @@ Definition msg1_spec nA pkA :=
   TPair (TInt 1) (TPair nA (TPair pkA (TInt 0))).
 
 Definition msg1_pred p : iProp Σ :=
-  ∃ nA kA, ⌜p.2 = Spec.of_list [nA; TKey Enc (TNonce kA)]⌝ ∗
+  ∃ nA kA, ⌜p.2 = Spec.of_list [nA; TKey Enc kA]⌝ ∗
            term_session_frag nA (Session Init kA p.1 None).
 
 Global Instance msg1_pred_proper : NonExpansive msg1_pred.
@@ -333,7 +333,7 @@ Proof. apply _. Qed.
 
 Definition msg2_pred p : iProp Σ :=
   ∃ nA nB kB,
-    ⌜p.2 = Spec.of_list [nA; nB; TKey Enc (TNonce kB)]⌝ ∗
+    ⌜p.2 = Spec.of_list [nA; nB; TKey Enc kB]⌝ ∗
     term_session_frag nB (Session Resp p.1 kB (Some nA)).
 
 Global Instance msg2_pred_proper : NonExpansive msg2_pred.
@@ -403,10 +403,12 @@ Definition role_name rl : gname :=
   if rl is Init then nsl_init_name else nsl_resp_name.
 
 Definition nsl_key rl k : iProp Σ :=
+  termT Pub (TKey Enc k) ∗
+  stermT Sec (TKey Dec k) ∗
   match rl with
-  | Init => tag_akeyT Pub "m2" (OfeMor msg2_pred) k
-  | Resp => tag_akeyT Pub "m1" (OfeMor msg1_pred) k ∗
-            tag_akeyT Pub "m3" (OfeMor msg3_pred) k
+  | Init => tkey_predT "m2" (OfeMor msg2_pred) k
+  | Resp => tkey_predT "m1" (OfeMor msg1_pred) k ∗
+            tkey_predT "m3" (OfeMor msg3_pred) k
   end.
 Arguments nsl_key : simpl never.
 
@@ -414,12 +416,8 @@ Global Instance nsl_key_persistent rl k :
   Persistent (nsl_key rl k).
 Proof. rewrite /nsl_key; case: rl; apply _. Qed.
 
-Lemma nsl_key_pub rl k : nsl_key rl k -∗ pub_enc_key k.
-Proof.
-rewrite /nsl_key; case: rl => /=.
-- iIntros "[H _]"; iExists _, _; eauto.
-- iIntros "[[H _] _]"; iExists _, _; eauto.
-Qed.
+Lemma nsl_key_pub rl k : nsl_key rl k -∗ termT Pub (TKey Enc k).
+Proof. by iDestruct 1 as "[??]". Qed.
 
 Definition coherent_views SM t1 s1 : Prop :=
   match s1.(srole), s1.(sdata) with
@@ -468,7 +466,7 @@ Lemma nsl_sess_alloc lvl kI kR t rl E ot :
   nsl_ctx -∗
   nsl_key rl kA -∗
   unregistered t -∗
-  pub_enc_key kB -∗
+  termT Pub (TKey Enc kB) -∗
   guarded lvl (nsl_key (swap_role rl) kB) -∗
   stermT lvl t -∗
   (if ot is Some t' then stermT lvl t' else True) ={E}=∗
@@ -513,7 +511,7 @@ Lemma nsl_sess_alloc_init lvl kA kB tA E :
   nsl_ctx -∗
   nsl_key Init kA -∗
   unregistered tA -∗
-  pub_enc_key kB -∗
+  termT Pub (TKey Enc kB) -∗
   guarded lvl (nsl_key Resp kB) -∗
   stermT lvl tA ={E}=∗
   guarded lvl (term_session_auth tA (Session Init kA kB None) ∗
@@ -528,7 +526,7 @@ Lemma nsl_sess_alloc_resp lvl kA kB tA tB E :
   nsl_ctx -∗
   nsl_key Resp kB -∗
   unregistered tB -∗
-  pub_enc_key kA -∗
+  termT Pub (TKey Enc kA) -∗
   guarded lvl (nsl_key Init kA) -∗
   stermT lvl tB -∗
   stermT lvl tA ={E}=∗
@@ -649,15 +647,14 @@ Qed.
 Lemma term_session_session_inv3 E lvl t s :
   ↑cryptoN.@"nsl" ⊆ E →
   nsl_ctx -∗
-  termT lvl (TKey Enc (TNonce (sowner s))) -∗
+  termT lvl (TKey Enc (sowner s)) -∗
   guarded lvl (term_session_frag t s) ={E}=∗
-  ▷ pub_enc_key (sowner s).
+  ▷ termT Pub (TKey Enc (sowner s)).
 Proof.
 iIntros (sub) "#Hctx #Ht #Hsess".
 iMod (term_session_session_inv0 with "Hctx Hsess") as (s') "[%s_s' Hs']" => //.
 iDestruct "Hs'" as "(#Hk&_)".
 case: lvl=> //=; do 2!iModIntro.
-  by iApply termT_TAEncE.
 rewrite /sowner.
 case/to_session_included: s_s' => [] <- [] <- [] <- _.
 by iApply nsl_key_pub.
@@ -796,18 +793,18 @@ Hypothesis wp_gen : forall E lvl Ψ,
 Lemma termT_msg1 lvl kA kB (tA : term) :
   nsl_key Init kA -∗
   stermT lvl tA -∗
-  pub_enc_key kB -∗
+  termT Pub (TKey Enc kB) -∗
   guarded lvl (nsl_key Resp kB) -∗
   guarded lvl (term_session_frag tA (Session Init kA kB None)) -∗
-  termT Pub (TEnc (TNonce kB) (Spec.tag "m1" (Spec.of_list [tA; TKey Enc (TNonce kA)]))).
+  termT Pub (TEnc kB (Spec.tag "m1" (Spec.of_list [tA; TKey Enc kA]))).
 Proof.
-iIntros "#HkA #HtA #HkB_lo (#HkB_hi & _) #frag".
+iIntros "#HkA #HtA #HkB_lo (#HkB_hi & #HkB_hi' & #? & _) #frag".
 iApply termT_tag_aenc_pub_secG; eauto.
   iApply termT_of_list => /=.
   iSplit; first by iDestruct "HtA" as "[??]".
   iSplit => //.
-  iApply (@sub_termT _ _ _ Pub) => //.
-  by iDestruct "HkA" as "[HkA _]"; iApply termT_TAEnc.
+  iApply (@sub_termT _ _ Pub) => //.
+  by iDestruct "HkA" as "[HkA _]".
 case: lvl => //=; iModIntro; by iExists _, _; eauto.
 Qed.
 
@@ -820,7 +817,7 @@ Lemma wp_initiator kA kB (tA : term) lvl E Ψ :
   stermT lvl tA -∗
   unregistered tA -∗
   nsl_key Init kA -∗
-  pub_enc_key kB -∗
+  termT Pub (TKey Enc kB) -∗
   guarded lvl (nsl_key Resp kB) -∗
   (∀ onB : option term,
       (if onB is Some tB then
@@ -831,7 +828,7 @@ Lemma wp_initiator kA kB (tA : term) lvl E Ψ :
          )
        else True) -∗
       Ψ (repr onB)) -∗
-  WP initiator (TKey Dec (TNonce kA)) (TKey Enc (TNonce kA)) (TKey Enc (TNonce kB)) tA #() @ E
+  WP initiator (TKey Dec kA) (TKey Enc kA) (TKey Enc kB) tA #() @ E
      {{ Ψ }}.
 Proof.
 rewrite /initiator.
@@ -852,8 +849,9 @@ wp_lookup pkB' epkB'; last protocol_failure.
 wp_eq_term e; last protocol_failure; subst nA'.
 wp_eq_term e; last protocol_failure; subst pkB'.
 wp_tenc.
-iDestruct (termT_tag_adec_pub_sec with "Hm2 [//]") as (lm2) "{Hm2} [#Hm2 #fragB]".
-iPoseProof (termT_of_listE with "Hm2") as "{Hm2} Hm2".
+iDestruct (termT_tag_adec_pub_sec with "Hm2 []") as (lm2) "{Hm2} [#Hm2 #fragB]".
+  by iDestruct "HkA" as "(?&?&?)".
+rewrite termT_of_list.
 iPoseProof (big_sepL_lookup with "Hm2") as "m2_tA"; first exact: enA'.
 iPoseProof (big_sepL_lookup with "Hm2") as "m2_nB"; first exact: enB.
 iPoseProof (big_sepL_lookup with "Hm2") as "m2_kB"; first exact: epkB'.
@@ -872,13 +870,13 @@ iAssert (▷ ⌜lm2 = lvl⌝)%I as "e".
   iModIntro.
   case: lvl lm2 Hlm2 => [] // [] //= _.
   iDestruct "sessB" as "(_&_&_&_&HtA')".
-  by iApply (stermT_eq with "HtA' HtA").
+  by iApply (stermT_eq' with "HtA' HtA").
 wp_pures; iDestruct "e" as "->".
 iMod (nsl_sess_update with "Hctx auth fragB") as "{fragA} [auth #fragA]" => //.
 set m3 := TEnc _ _.
 wp_bind (send _); iApply wp_send.
   iModIntro.
-  iDestruct "HkB_hi" as "(HkB_m1 & HhB_m3)".
+  iDestruct "HkB_hi" as "(HkB_m1 & HkB_m3 & ? & ?)".
   iApply (termT_tag_aenc_pub_secG _ lvl) => //; eauto.
   by case: (lvl) => //=; iModIntro; iExists tA, kA; iSplit.
 wp_pures; iApply ("Hpost" $! (Some nB)).
@@ -895,14 +893,6 @@ Lemma sub_termT_pub lvl t : termT Pub t -∗ termT lvl t.
 Proof. by iApply sub_termT. Qed.
 (* /MOVE *)
 
-Lemma termT_TKeyE lvl kt t :
-  termT lvl (TKey kt t) -∗
-  ∃ k, ⌜t = TNonce k⌝.
-Proof.
-iIntros "H"; rewrite termT_eq /=.
-by case: t => [] // k; eauto.
-Qed.
-
 Lemma wp_responder kB E Ψ :
   ↑cryptoN.@"nsl" ⊆ E →
   nsl_ctx -∗
@@ -910,8 +900,8 @@ Lemma wp_responder kB E Ψ :
   (∀ ot : option (term * term * term),
       (if ot is Some (pkA, nA, nB) then
          ∃ lvl kA,
-           ⌜pkA = TKey Enc (TNonce kA)⌝ ∗
-           pub_enc_key kA ∗
+           ⌜pkA = TKey Enc kA⌝ ∗
+           termT Pub pkA ∗
            stermT lvl nA ∗
            stermT lvl nB ∗
            guarded lvl (
@@ -919,7 +909,7 @@ Lemma wp_responder kB E Ψ :
             term_session_auth nB (Session Resp kA kB (Some nA)))
        else True) -∗
        Ψ (repr ot)) -∗
-  WP responder (TKey Dec (TNonce kB)) (TKey Enc (TNonce kB)) #() @ E {{ Ψ }}.
+  WP responder (TKey Dec kB) (TKey Enc kB) #() @ E {{ Ψ }}.
 Proof.
 iIntros (?) "#Hctx #HkB Hpost".
 rewrite /responder; wp_pures.
@@ -928,16 +918,15 @@ wp_tdec m1; last protocol_failure.
 wp_list_of_term m1; last protocol_failure.
 wp_lookup nA enA; last protocol_failure.
 wp_lookup pkA epkA; last protocol_failure.
-wp_is_key_eq kt kA' et; last protocol_failure; subst pkA.
+wp_is_key_eq kt kA et; last protocol_failure; subst pkA.
 wp_pures.
 case: (bool_decide_reflect (_ = repr_key_type Enc)); last protocol_failure.
 case: kt epkA=> // epkA _.
-iPoseProof "HkB" as "(HkB_m1 & HkB_m3)".
-iDestruct (termT_tag_adec_pub_sec with "Hm1 [//]") as (lm1) "{Hm1} [Hm1 fragA]".
-iPoseProof (termT_of_listE with "Hm1") as "{Hm1} Hm1".
+iPoseProof "HkB" as "(? & ? & HkB_m1 & HkB_m3)".
+iDestruct (termT_tag_adec_pub_sec with "Hm1 []") as (lm1) "{Hm1} [Hm1 fragA]"; eauto.
+rewrite termT_of_list.
 iPoseProof (big_sepL_lookup with "Hm1") as "HnA"; first exact: enA.
 iPoseProof (big_sepL_lookup with "Hm1") as "HpkA"; first exact: epkA.
-iDestruct (termT_TKeyE with "HpkA") as (kA) "->".
 pose Pm1 := term_session_frag nA (Session Init kA kB None).
 iAssert (guarded lm1 Pm1) as "{fragA} fragA".
   iApply (guarded_mono with "fragA").
@@ -952,16 +941,17 @@ wp_pures; wp_bind (gen _); iApply (wp_gen _ lm1); iIntros (nB) "unreg #HnB".
 wp_pures.
 wp_list (_ :: _ :: _ :: []); wp_term_of_list. 
 wp_tenc; wp_pures.
-set m2 := Spec.of_list [nA; nB; TKey Enc (TNonce kB)].
+set m2 := Spec.of_list [nA; nB; TKey Enc kB].
 set sB := Session Resp kA kB (Some nA).
 iMod (nsl_sess_alloc_resp _ kA kB nA with "Hctx HkB unreg HkA_lo HkA_hi HnB HnA")
     as "[auth #fragB]"=> //=.
 wp_bind (send _); iApply wp_send.
   iModIntro.
+  iDestruct "HkA_hi" as "(?&?&?)".
   iApply termT_tag_aenc_pub_secG; eauto.
     iApply termT_of_list => /=.
     do !iSplit => //; try by iApply stermT_termT.
-    by iApply sub_termT_pub; iApply termT_TAEnc; iDestruct "HkB_m1" as "[??]".
+    by iApply sub_termT_pub.
   case: lm1 => //=; iModIntro.
   by iExists nA, nB, kB; iSplit; first trivial.
 wp_pures; wp_bind (recv _); iApply wp_recv; iIntros (m3) "#Hm3".
